explicit proof structure in Ackermann/fol.v, folProof.v, folProp.v

theories/ordinals/Ackermann/folProof.v
@@ -1,6 +1,4 @@
-Require Import Ensembles.
-Require Import Coq.Lists.List.
-Require Import Arith.
+From Coq Require Import Ensembles Lists.List Arith. 
 
 Require Export fol.
 Require Import folProp.
@@ -23,81 +21,75 @@ Let notH := notH L.
 Let iffH := iffH L.
 Let forallH := forallH L.
 
-Definition nVars (n : nat) : Terms n * Terms n.
-intros.
-induction n as [| n Hrecn].
-split.
-exact (Tnil L).
-exact (Tnil L).
-induction Hrecn as (a, b).
-split.
-constructor.
-exact (var (n + n)).
-exact a.
-constructor.
-exact (var (S (n + n))).
-exact b.
-Defined.
+Fixpoint nVars (n: nat) : Terms n * Terms n:=
+  match n with 
+    0 => (Tnil L, Tnil L)
+  | S n0 => 
+      (let (a,b) := nVars n0 in
+       (Tcons L n0 (var (n0 + n0)) a, Tcons L n0 (var (S (n0 + n0))) b))
+  end.
+
+
 
 Definition AxmEq4 (R : Relations L) : Formula.
-intros.
-assert (forall (f : Formula) (n : nat), Formula).
-intros.
-induction n as [| n Hrecn].
-exact f.
-exact (impH (equal (var (n + n)) (var (S (n + n)))) Hrecn).
-apply H.
-induction (nVars (arity L (inl _ R))).
-apply (iffH (atomic R a) (atomic R b)).
-apply (arity L (inl _ R)).
+Proof. 
+  assert (X: forall (f : Formula) (n : nat), Formula).
+  { intros f n; induction n as [| n Hrecn].
+    - exact f.
+    - exact (impH (equal (var (n + n)) (var (S (n + n)))) Hrecn).
+  } 
+  apply X.
+  - induction (nVars (arity L (inl _ R))).
+    apply (iffH (atomic R a) (atomic R b)).
+  - apply (arity L (inl _ R)).
 Defined.
 
 Definition AxmEq5 (f : Functions L) : Formula.
-intros.
-assert (forall (f : Formula) (n : nat), Formula).
-intros.
-induction n as [| n Hrecn].
-exact f0.
-exact (impH (equal (var (n + n)) (var (S (n + n)))) Hrecn).
-apply H.
-induction (nVars (arity L (inr _ f))).
-apply (equal (apply f a) (apply f b)).
-apply (arity L (inr _ f)).
+Proof. 
+  assert (X: forall (f : Formula) (n : nat), Formula).
+  { intros f0 n; induction n as [| n Hrecn].
+    - exact f0.
+    - exact (impH (equal (var (n + n)) (var (S (n + n)))) Hrecn).
+  } 
+  apply X.
+  induction (nVars (arity L (inr _ f))) as [a b].
+  - apply (equal (apply f a) (apply f b)).
+  - apply (arity L (inr _ f)).
 Defined.
 
 Inductive Prf : Formulas -> Formula -> Set :=
-  | AXM : forall A : Formula, Prf (A :: nil) A
-  | MP :
-      forall (Axm1 Axm2 : Formulas) (A B : Formula),
-      Prf Axm1 (impH A B) -> Prf Axm2 A -> Prf (Axm1 ++ Axm2) B
-  | GEN :
-      forall (Axm : Formulas) (A : Formula) (v : nat),
-      ~ In v (freeVarListFormula L Axm) -> Prf Axm A -> Prf Axm (forallH v A)
-  | IMP1 : forall A B : Formula, Prf nil (impH A (impH B A))
-  | IMP2 :
-      forall A B C : Formula,
-      Prf nil (impH (impH A (impH B C)) (impH (impH A B) (impH A C)))
-  | CP :
-      forall A B : Formula,
-      Prf nil (impH (impH (notH A) (notH B)) (impH B A))
-  | FA1 :
-      forall (A : Formula) (v : nat) (t : Term),
-      Prf nil (impH (forallH v A) (substituteFormula L A v t))
-  | FA2 :
-      forall (A : Formula) (v : nat),
-      ~ In v (freeVarFormula L A) -> Prf nil (impH A (forallH v A))
-  | FA3 :
-      forall (A B : Formula) (v : nat),
-      Prf nil
-        (impH (forallH v (impH A B)) (impH (forallH v A) (forallH v B)))
-  | EQ1 : Prf nil (equal (var 0) (var 0))
-  | EQ2 : Prf nil (impH (equal (var 0) (var 1)) (equal (var 1) (var 0)))
-  | EQ3 :
-      Prf nil
-        (impH (equal (var 0) (var 1))
-           (impH (equal (var 1) (var 2)) (equal (var 0) (var 2))))
-  | EQ4 : forall R : Relations L, Prf nil (AxmEq4 R)
-  | EQ5 : forall f : Functions L, Prf nil (AxmEq5 f).
+| AXM : forall A : Formula, Prf (A :: nil) A
+| MP :
+  forall (Axm1 Axm2 : Formulas) (A B : Formula),
+    Prf Axm1 (impH A B) -> Prf Axm2 A -> Prf (Axm1 ++ Axm2) B
+| GEN :
+  forall (Axm : Formulas) (A : Formula) (v : nat),
+    ~ In v (freeVarListFormula L Axm) -> Prf Axm A -> Prf Axm (forallH v A)
+| IMP1 : forall A B : Formula, Prf nil (impH A (impH B A))
+| IMP2 :
+  forall A B C : Formula,
+    Prf nil (impH (impH A (impH B C)) (impH (impH A B) (impH A C)))
+| CP :
+  forall A B : Formula,
+    Prf nil (impH (impH (notH A) (notH B)) (impH B A))
+| FA1 :
+  forall (A : Formula) (v : nat) (t : Term),
+    Prf nil (impH (forallH v A) (substituteFormula L A v t))
+| FA2 :
+  forall (A : Formula) (v : nat),
+    ~ In v (freeVarFormula L A) -> Prf nil (impH A (forallH v A))
+| FA3 :
+  forall (A B : Formula) (v : nat),
+    Prf nil
+      (impH (forallH v (impH A B)) (impH (forallH v A) (forallH v B)))
+| EQ1 : Prf nil (equal (var 0) (var 0))
+| EQ2 : Prf nil (impH (equal (var 0) (var 1)) (equal (var 1) (var 0)))
+| EQ3 :
+  Prf nil
+    (impH (equal (var 0) (var 1))
+       (impH (equal (var 1) (var 2)) (equal (var 0) (var 2))))
+| EQ4 : forall R : Relations L, Prf nil (AxmEq4 R)
+| EQ5 : forall f : Functions L, Prf nil (AxmEq5 f).
 
 Definition SysPrf (T : System) (f : Formula) :=
   exists Axm : Formulas,
